axiomatic/theories/core/uvar.thy
@@ -18,6 +18,11 @@ no_notation
   Set.member ("op :") and
   Set.member ("(_/ : _)" [51, 51] 50)
 
+text {* We are going to use the converse symbol for undashing. *}
+
+no_notation
+  converse  ("(_\<inverse>)" [1000] 999)
+
 default_sort typerep
 
 text {* Avoids verbose printing of the prefix in @{text "'a uvar.var"}. *}
@@ -204,6 +209,37 @@ definition undash_var :: "'a var \<Rightarrow> 'a var" where
 
 adhoc_overloading undash undash_var
 
+subsection {* Proof Support *}
+
+text {*
+  To facilitate proofs about variables, we configure tactics that automatically
+  apply transfer laws for the types @{type var}, @{type uvar} and @{type uname}.
+  While record-based types already generate the underlying splitting laws, for
+  the @{type var} type being defined via a type definition, we make use of the
+  utility theory @{theory Typedef_extra} which generates those laws for us.
+*}
+
+subsubsection {* Transfer Laws *}
+
+text {* Using a named attribute supports future extension. *}
+
+named_theorems var_transfer "variable transfer"
+
+lemmas var_typedef_transfer =
+  type_definition.transfer [OF uvar.type_definition_var]
+
+declare uname.uname.splits [var_transfer]
+declare uvar.uvar.splits [var_transfer]
+declare var_typedef_transfer [var_transfer]
+
+subsubsection {* Proof Methods *}
+
+text {* The below automates, in particular, laws about variable decorations. *}
+
+method var_tac = (clarsimp simp add: var_transfer vars typing fun_eq_iff)
+method var_auto = (var_tac; auto)
+method var_blast = (var_tac; blast)
+
 subsubsection {* Theorems *}
 
 lemma p_type_of_Rep_var [simp]:
@@ -212,6 +248,16 @@ fixes v :: "'a var"
 shows "x : (type v\<down>)"
 apply (transfer)
 apply (simp add: typing)
+done
+
+lemma undash_uvar_inv [simp]:
+"(v::uvar) \<in> DASHED \<Longrightarrow> v\<inverse>\<acute> = v"
+apply (var_tac)
+done
+
+lemma dash_uvar_inv [simp]:
+"(v::uvar) \<in> UNDASHED \<Longrightarrow> v\<acute>\<inverse> = v"
+apply (var_tac)
 done
 
 lemma dash_erasure_commutes:
