axiomatic/theories/utils/Interpret.thy
@@ -1,0 +1,114 @@
+(******************************************************************************)
+(* Project: The Isabelle/UTP Proof System                                     *)
+(* File: Interpret.thy                                                        *)
+(* Authors: Simon Foster and Frank Zeyda                                      *)
+(* Emails: simon.foster@york.ac.uk frank.zeyda@york.ac.uk                     *)
+(******************************************************************************)
+(* LAST REVIEWED: 15 Feb 2017 *)
+
+section {* Interpretation Tools *}
+
+theory Interpret
+imports Main
+begin
+
+subsection {* Preliminaries *}
+
+definition surj_on :: "('a \<Rightarrow> 'b) \<Rightarrow> 'a set \<Rightarrow> bool" where
+"surj_on f A \<longleftrightarrow> f ` A = UNIV"
+
+lemma surj_onI [intro]:
+"f ` A = UNIV \<Longrightarrow> surj_on f A"
+apply (unfold surj_on_def)
+apply (assumption)
+done
+
+lemma surj_onD [dest]:
+"surj_on f A \<Longrightarrow> \<exists>x\<in>A. f x = y"
+apply (unfold surj_on_def)
+apply (simp add: image_def)
+apply (simp add: set_eq_iff)
+apply (drule_tac x = "y" in spec)
+apply (clarsimp)
+apply (rule_tac x = "x" in bexI)
+apply (rule refl)
+apply (assumption)
+done
+
+lemma surj_comp_funct:
+"inj f \<Longrightarrow> surj (\<lambda>g. g o f)"
+apply (rule_tac f = "\<lambda>g. g o (inv f)" in surjI)
+apply (simp)
+done
+
+subsection {* Locale @{text interp} *}
+
+text {*
+  Interestingly, surjectivity of the interpretation function @{term f} turns
+  out to be sufficient. Compare this, for instance, to the assumptions used in
+  the theory @{text Transfer_extra} where we effectively exploit the fact that
+  the abstraction and representation functions are indeed mutual inverses.
+*}
+
+locale interp =
+fixes f :: "'a \<Rightarrow> 'b"
+fixes A :: "'a set"
+assumes f_surj_on_A: "surj_on f A"
+begin
+lemma forall_transfer:
+"(\<forall>y::'b. P y) = (\<forall>(x::'a)\<in>A. P (f x))"
+apply (safe)
+-- {* Subgoal 1 *}
+apply (drule_tac x = "f x" in spec)
+apply (assumption)
+-- {* Subgoal 2 *}
+apply (insert surj_onD [OF f_surj_on_A])
+apply (drule_tac x = "y" in meta_spec)
+apply (clarsimp)
+done
+
+lemma exists_transfer:
+"(\<exists>y::'b. P y) = (\<exists>(x::'a)\<in>A. P (f x))"
+apply (safe)
+-- {* Subgoal 1 *}
+apply (insert surj_onD [OF f_surj_on_A]) [1]
+apply (drule_tac x = "y" in meta_spec)
+apply (clarsimp)
+apply (rule_tac x = "x" in bexI)
+apply (assumption)
+apply (assumption)
+-- {* Subgoal 2 *}
+apply (rule_tac x = "f x" in exI)
+apply (assumption)
+done
+
+lemma meta_transfer:
+"(\<And>y::'b. PROP P y) \<equiv> (\<And>x::'a. x \<in> A \<Longrightarrow> PROP P (f x))"
+apply (rule)
+-- {* Subgoal 1 *}
+apply (drule_tac x = "f x" in meta_spec)
+apply (assumption)
+-- {* Subgoal 2 *}
+apply (insert surj_onD [OF f_surj_on_A])
+apply (drule_tac x = "y" in meta_spec)
+(* apply (clarsimp) *)
+(* The following is clumsy but clarsimp seems not to work?! *)
+apply (drule_tac x = "SOME x. x \<in> A \<and> f x = y" in meta_spec)
+apply (subgoal_tac "(SOME x. x \<in> A \<and> f x = y) \<in> A")
+-- {* Subgoal 2.1 *}
+apply (clarsimp)
+apply (subgoal_tac "f (SOME x. x \<in> A \<and> f x = y) = y")
+-- {* Subgoal 2.1.1 *}
+apply (clarsimp)
+-- {* Subgoal 2.1.2 *}
+apply (erule someI2_bex; clarsimp)
+-- {* Subgoal 2.2 *}
+apply (erule someI2_bex; clarsimp)
+done
+
+lemmas transfer =
+  meta_transfer
+  forall_transfer
+  exists_transfer
+end
+end
