ROOT
@@ -19,7 +19,7 @@ session "HOL-Algebra2" (main timing) in "contrib/Algebra" = HOL +
     "~~/src/HOL/Number_Theory/Primes"
     "~~/src/HOL/Library/Permutation"
   theories [document = pdf]
-    (*** New development, based on explicit structures ***)    
+    (*** New development, based on explicit structures ***)
     (* Groups *)
     FiniteProduct        (* Product operator for commutative groups *)
     Sylow                (* Sylow's theorem *)
@@ -37,7 +37,7 @@ session "HOL-Algebra2" (main timing) in "contrib/Algebra" = HOL +
     UnivPoly             (* Polynomials *)
   document_files "root.bib" "root.tex"
 
-(* Kleene Algebra *)    
+(* Kleene Algebra *)
 
 session Kleene_Algebra (AFP) in "contrib/Kleene_Algebra"
   = "HOL-Library" +
@@ -59,8 +59,8 @@ session Kleene_Algebra (AFP) in "contrib/Kleene_Algebra"
     "document/root.tex"
 
 (* Lenses *)
-    
-session "Optics" in "lenses" 
+
+session "Optics" in "lenses"
   = "HOL-Algebra2" +
   options [timeout = 300]
   theories
@@ -73,7 +73,7 @@ session "Optics" in "lenses"
     Lenses
 
 (* Continuum Universe *)
-    
+
 session "Continuum" in "continuum" = "HOL-Cardinals" +
   options [document = false, timeout = 1000]
   theories
@@ -85,16 +85,16 @@ session "Continuum" in "continuum" = "HOL-Cardinals" +
     Real_Bit
     UNIV_TYPE
 
-(* Continuous system dynamics *)
-    
+(* Continuous System Dynamics *)
+
 session "Dynamics" in "dynamics" = "HOL-Analysis" +
   options [document = false, timeout = 1000]
   theories
     Derivative_extra
     Contiguous_Functions
     Timed_Traces
-    
-(* UTP library imports *)
+
+(* Library Imports for UTP *)
 
 session "UTP-IMPORTS" in "utils" = "Optics" +
   options [document = false, timeout = 1000]
@@ -115,13 +115,24 @@ session "UTP-IMPORTS" in "utils" = "Optics" +
     "Library_extra/Pfun"
     "Library_extra/Ffun"
 
-(* Imports including the axiomatic value model *)
+(* Library Imports for UTP-AX *)
 
 session "UTP-IMPORTS-AX" in "axiomatic/theories" = "UTP-IMPORTS" +
   options [browser_info = true, document = false]
-  theories "core/ulens" "core/udefaults"
+  theories
+    "uimports"
+    "ucommon"
+    "core/uconsts"
+    "core/uname"
+    "core/utype"
+    "core/uval"
+    "core/uvar"
+    "core/ustate"
+    "core/ustore"
+    "core/ulens"
+    "core/udefaults"
 
-(* Core UTP framework *)
+(* UTP Core Framework *)
 
 session "UTP" in "utp" = "UTP-IMPORTS" +
   options [document = pdf, document_output = "output", timeout = 1000]
@@ -132,15 +143,15 @@ session "UTP" in "utp" = "UTP-IMPORTS" +
     "root.tex"
     "document.sty"
 
-(* Imports including deep variables *)
-    
+(* Core UTP with Deep Variables *)
+
 session "UTP-DEEP" in "deep" = "UTP" +
   options [browser_info = true, document = false]
   theories
     "../continuum/Continuum"
     utp_deep
-    
-(* Core framework including the axiomatic value model *)
+
+(* Core UTP with Axiomatic Variables *)
 
 session "UTP-AX" in "utp" = "UTP-IMPORTS-AX" +
   options [document = pdf, document_output = "output", timeout = 1000]
@@ -153,9 +164,9 @@ session "UTP-AX" in "utp" = "UTP-IMPORTS-AX" +
 
 (* Imports for Hybrid UTP *)
 
-(* We chose to start another root from the Analysis session (via Dynamics) 
-   and build everything else on top of it. This is because Analysis takes 
-   more than 10 minutes to build on a laptop and everything else is 
+(* We chose to start another root from the Analysis session (via Dynamics)
+   and build everything else on top of it. This is because Analysis takes
+   more than 10 minutes to build on a laptop and everything else is
    comparatively lightweight. *)
 
 session "UTP-HY-IMPORTS" = "Dynamics" +
@@ -182,3 +193,14 @@ session "VDM-SL" in "vdm-sl" = "UTP-DEEP" +
   theories
     PFOL
     VDM
+
+(* FMI Mechanisation *)
+
+session "FMI" in "fmi" = "UTP-AX" +
+  options [document = pdf, document_output = "output", timeout = 1000]
+  theories
+    fmi
+  document_files
+    "root.tex"
+    (* "root.bib" *)
+    "document.sty"
