build.sh
@@ -1,7 +1,19 @@
 #!/bin/sh
-isabelle build -c -b UTP-DEPS
+isabelle build -c -b HOL-Algebra2
+# Session Kleene_Algebra does not seem to compile. Talk to Simon!
+#isabelle build -c -b Kleene_Algebra
+isabelle build -c -b Optics
+isabelle build -c -b Continuum
+isabelle build -c -b Dynamics
 isabelle build -c -b UTP-IMPORTS
 isabelle build -c -b UTP-IMPORTS-AX
 isabelle build -c -b UTP
+isabelle build -c -b UTP-DEEP
 isabelle build -c -b UTP-AX
+# Session UTP-HY-IMPORTS does not seem to compile. Talk to Simon!
+#isabelle build -c -b UTP-HY-IMPORTS
+# Session UTP-Hybrid does not seem to compile.  Talk to Simon!
+#isabelle build -c -b UTP-Hybrid
 isabelle build -c -b VDM-SL
+# Session FMI will be integrated with the subsequent merge with master.
+#isabelle build -c -b FMI
